theories/Symbolic/OccursCheck.v
@@ -27,9 +27,6 @@
 (* SOFTWARE, EVEN IF ADVISED OF THE POSSIBILITY OF SUCH DAMAGE.               *)
 (******************************************************************************)
 
-From Coq Require Import
-     Program.Tactics.
-
 From Equations Require Import
      Equations.
 From Katamaran Require Import
@@ -44,6 +41,8 @@ From Katamaran Require Import
 
 Import ctx.notations.
 Import env.notations.
+Import option.
+Import option.notations.
 
 Local Set Implicit Arguments.
 
@@ -55,252 +54,171 @@ Module Type OccursCheckOn
   Local Notation LCtx := (NCtx 𝑺 Ty).
 
   Class OccursCheck (T : LCtx -> Type) : Type :=
-    occurs_check : forall {Σ x} (xIn : x ∈ Σ) (t : T Σ), option (T (Σ - x)%ctx).
-  Class OccursCheckLaws (T : LCtx -> Type) `{Subst T, OccursCheck T} : Prop :=
-    { occurs_check_shift {Σ x σ} (xIn : x∷σ ∈ Σ) (t : T (Σ - x∷σ)) :
-        occurs_check xIn (subst t (sub_shift xIn)) = Some t;
-      occurs_check_sound {Σ x} (xIn : x ∈ Σ) (t : T Σ) (t' : T (Σ - x)) :
-        occurs_check xIn t = Some t' -> t = subst t' (sub_shift xIn);
-    }.
-  Global Arguments OccursCheckLaws T {_ _}.
+    occurs_check : forall {Σ x} (xIn : x ∈ Σ) (t : T Σ), option (T (Σ - x)).
 
-  Import stdpp.base.
+  #[export] Instance occurs_check_env {I : Set} {T : LCtx -> I -> Set}
+         {OCT : forall i, OccursCheck (fun Σ => T Σ i)} :
+    forall {Γ : Ctx I}, OccursCheck (fun Σ => Env (T Σ) Γ) :=
+    fix oc {Γ Σ x} xIn ts {struct ts} :=
+      match ts with
+      | env.nil         => Some env.nil
+      | env.snoc ts _ t =>
+          ts' <- occurs_check (OccursCheck := @oc _) xIn ts;;
+          t'  <- occurs_check xIn t;;
+          Some (env.snoc ts' _ t')
+      end.
 
-  Fixpoint occurs_check_term {Σ x} (xIn : x ∈ Σ) {σ} (t : Term Σ σ) : option (Term (Σ - x) σ) :=
-    match t with
-    | @term_var _ ς σ0 ςInΣ =>
-      match ctx.occurs_check_var xIn ςInΣ with
-      | inl e     => None
-      | inr ςInΣ' => Some (@term_var _ _ _ ςInΣ')
-      end
-    | term_val σ0 v => Some (term_val σ0 v)
-    | term_binop op t1 t2 =>
-      t1' ← occurs_check_term xIn t1; t2' ← occurs_check_term xIn t2; Some (term_binop op t1' t2')
-    | term_neg t => option_map term_neg (occurs_check_term xIn t)
-    | term_not t => option_map term_not (occurs_check_term xIn t)
-    | term_inl t => option_map term_inl (occurs_check_term xIn t)
-    | term_inr t => option_map term_inr (occurs_check_term xIn t)
-    | @term_projtup _ σs t n σ p =>
-      option_map (fun t' => @term_projtup _ _ t' n _ p) (occurs_check_term xIn t)
-    | term_union U K t => option_map (term_union U K) (occurs_check_term xIn t)
-    | term_record R es => option_map (term_record R) (env.traverse (fun _ => occurs_check_term xIn) es)
-    (* | term_projrec t rf => option_map (fun t' => term_projrec t' rf) (occurs_check_term xIn t) *)
-    end.
+  #[export] Instance occurs_check_term : forall σ, OccursCheck (fun Σ => Term Σ σ) :=
+    fix occurs_check_term {τ Σ x} xIn (t : Term Σ τ) {struct t} : option (Term (Σ - x) τ) :=
+      match t with
+      | @term_var _ y _ yIn => match ctx.occurs_check_var xIn yIn with
+                              | inl _    => None
+                              | inr yIn' => Some (term_var y)
+                              end
+      | term_val σ v => Some (term_val σ v)
+      | term_binop op t1 t2 =>
+          t1' <- occurs_check_term xIn t1;;
+          t2' <- occurs_check_term xIn t2;;
+          Some (term_binop op t1' t2')
+      | term_neg t => term_neg <$> occurs_check_term xIn t
+      | term_not t => term_not <$> occurs_check_term xIn t
+      | term_inl t => term_inl <$> occurs_check_term xIn t
+      | term_inr t => term_inr <$> occurs_check_term xIn t
+      | @term_projtup _ σs t n σ p =>
+        option.map (fun t' => @term_projtup _ _ t' n _ p) (occurs_check_term xIn t)
+      | term_union U K t0 => term_union U K <$> occurs_check_term xIn t0
+      | term_record R ts =>
+        let OCTerm xt := @occurs_check_term (@type 𝑹𝑭 Ty xt) in
+        term_record R <$> occurs_check (OccursCheck := occurs_check_env (OCT := OCTerm)) xIn ts
+      end.
 
-  Global Instance OccursCheckTerm {σ} : OccursCheck (fun Σ => Term Σ σ) :=
-    fun _ _ xIn => occurs_check_term xIn.
-
-  Global Instance OccursCheckList {T : LCtx -> Type} `{OccursCheck T} :
+  #[export] Instance occurs_check_list {T : LCtx -> Type} `{OccursCheck T} :
     OccursCheck (List T) :=
     fun _ _ xIn => traverse_list (occurs_check xIn).
 
-  Global Instance OccursCheckEnv {I : Set} {T : LCtx -> I -> Set}
-         {_ : forall i : I, OccursCheck (fun Σ => T Σ i)}
-         {Γ : Ctx I} :
-    OccursCheck (fun Σ => Env (T Σ) Γ) :=
-    fun _ _ xIn => env.traverse (fun i => occurs_check (T := fun Σ => T Σ i) xIn).
+  #[export] Instance occurs_check_sub {Σ} : OccursCheck (Sub Σ) :=
+    occurs_check_env.
 
-  Global Instance OccursCheckSub {Σ} : OccursCheck (Sub Σ) :=
-    OccursCheckEnv.
-
-  Lemma option_map_eq_some {A B} (f : A -> B) (o : option A) (a : A) :
-    o = Some a ->
-    option_map f o = Some (f a).
-  Proof. now intros ->. Qed.
-
-  Lemma option_map_eq_some' {A B} (f : A -> B) (o : option A) (b : B) :
-    option_map f o = Some b <->
-    exists a, o = Some a /\ f a = b.
-  Proof.
-    split.
-    - destruct o as [a|].
-      + intros H. apply noConfusion_inv in H. cbn in H.
-        exists a. split; congruence.
-      + discriminate.
-    - now intros (a & -> & <-).
-  Qed.
-
-  Lemma option_bind_eq_some {A B} (f : A -> option B) (o : option A) (b : B) :
-    (exists a, o = Some a /\ f a = Some b) <->
-    option.option_bind A B f o = Some b.
-  Proof.
-    split.
-    - now intros (a & -> & <-).
-    - destruct o as [a|]; [ now exists a | discriminate ].
-  Qed.
-
-  Local Ltac solve :=
-    repeat
-      match goal with
-      | H: Some _ = Some _ |- _ =>
-        apply noConfusion_inv in H; cbn in H; subst
-      | H: base.mbind _ _ = Some _ |- _ =>
-        apply option_bind_eq_some in H; cbn in H; destruct_conjs; subst
-      | H: option_map _ _ = Some _ |- _ =>
-        apply option_map_eq_some' in H; cbn in H; destruct_conjs; subst
-
-      | |- match occurs_check_term ?xIn ?t with _ => _ end = _ =>
-        destruct (occurs_check_term xIn t); try discriminate
-      | |- match occurs_check ?xIn ?t with _ => _ end = _ =>
-        destruct (occurs_check xIn t); try discriminate
-      | |- base.mbind _ _ = Some _ =>
-        apply option_bind_eq_some; eexists; split; [ eassumption; fail | idtac ]
-      | |- option_map ?f _ = Some (?f _) =>
-        apply option_map_eq_some
-      | |- option_map _ _ = Some _ =>
-        apply option_map_eq_some'; eexists; split; [ eassumption; fail | idtac ]
-      | |- _ =>
-        unfold base.mret, option.option_ret in *; cbn in *; try congruence
-      end.
-
-  Global Instance OccursCheckLawsTerm {τ} : OccursCheckLaws (fun Σ => Term Σ τ).
-  Proof.
-    constructor.
-    - intros; unfold occurs_check, OccursCheckTerm, subst, SubstTerm.
-      induction t; cbn.
-      + unfold sub_shift. rewrite env.lookup_tabulate.
-        cbv [occurs_check_term base.mbind option.option_bind].
-        now rewrite ctx.occurs_check_shift_var.
-      + solve.
-      + solve.
-      + solve.
-      + solve.
-      + solve.
-      + solve.
-      + solve.
-      + solve.
-      + solve.
-        induction es; destruct X; cbn.
-        * reflexivity.
-        * now rewrite IHes, e0.
-      (* + solve. *)
-    - unfold occurs_check, OccursCheckTerm, subst, SubstTerm.
-      intros ? ? ? t t' H1.
-      induction t; cbn in H1.
-      + pose proof (ctx.occurs_check_var_spec xIn ςInΣ) as H2.
-        destruct (ctx.occurs_check_var xIn ςInΣ); apply noConfusion_inv in H1;
-          cbn in H1; try contradiction; subst; cbn.
-        destruct H2 as [H2 H3]. subst. unfold sub_shift.
-        now rewrite env.lookup_tabulate.
-      + solve.
-      + solve. f_equal; auto.
-      + solve. f_equal; auto.
-      + solve. f_equal; auto.
-      + solve. f_equal; auto.
-      + solve. f_equal; auto.
-      + solve. f_equal. auto.
-      + solve. f_equal. auto.
-      + apply option_map_eq_some' in H1 as [ts [H ?]]. subst. cbn. f_equal.
-        change (es = subst ts (sub_shift xIn)).
-        induction es; destruct X; cbn.
-        * destruct (env.nilView ts). reflexivity.
-        * destruct (env.snocView ts).
-          change (es ► (b ↦ db) = subst E (sub_shift xIn) ► (b ↦ subst v (sub_shift xIn))).
-          cbn in H.
-          apply option.bind_Some in H.
-          destruct H as [E' [HE H]].
-          apply option.bind_Some in H.
-          destruct H as [t' [? Heq]].
-          unfold base.mret in Heq.
-          apply noConfusion_inv in Heq.
-          cbn in Heq.
-          apply env.inversion_eq_snoc in Heq.
-          destruct Heq; subst.
-          f_equal.
-          apply IHes; auto.
-          apply e0; auto.
-  Qed.
-
-  Global Instance OccursCheckLawsList {T : LCtx -> Type} `{OccursCheckLaws T} :
-    OccursCheckLaws (fun Σ => list (T Σ)).
-  Proof.
-    constructor.
-    - intros. induction t; cbn.
-      + reflexivity.
-      + cbv [base.mbind option.option_bind].
-        now rewrite occurs_check_shift, IHt.
-    - intros ? ? ? t. induction t; cbn; intros t' Heq.
-      + solve.
-      + solve. apply occurs_check_sound in H2.
-        f_equal; auto.
-  Qed.
-
-  Global Instance OccursCheckLawsEnv {I : Set} {T : LCtx -> I -> Set}
-         {_ : forall i : I, Subst (fun Σ => T Σ i)}
-         {_ : forall i : I, OccursCheck (fun Σ => T Σ i)}
-         {_ : forall i : I, OccursCheckLaws (fun Σ => T Σ i)}
-         {Γ : Ctx I} :
-    OccursCheckLaws (fun Σ => Env (T Σ) Γ).
-  Proof.
-    constructor.
-    - intros. induction t.
-      + reflexivity.
-      + unfold occurs_check, OccursCheckEnv, subst, SubstEnv in IHt.
-        cbn. cbv [base.mbind option.option_ret option.option_bind] in *.
-        now rewrite IHt, occurs_check_shift.
-    - intros ? ? ? E. induction E; cbn; intros E' Heq.
-      + solve. reflexivity.
-      + solve. apply (occurs_check_sound (T := fun Σ => T Σ _)) in H2.
-        f_equal.
-        * now apply IHE.
-        * auto.
-  Qed.
-
-  Global Instance OccursCheckLawsSub {Σ} : OccursCheckLaws (Sub Σ) :=
-    OccursCheckLawsEnv.
-
-  Global Instance OccursCheckPair {AT BT} `{OccursCheck AT, OccursCheck BT} :
+  #[export] Instance occurs_check_pair {AT BT} `{OccursCheck AT, OccursCheck BT} :
     OccursCheck (Pair AT BT) :=
     fun _ _ xIn '(a,b) =>
-      match occurs_check xIn a, occurs_check xIn b with
-      | Some a' , Some b' => Some (a', b')
-      | _       , _       => None
-      end.
+      a' <- occurs_check xIn a ;;
+      b' <- occurs_check xIn b ;;
+      Some (a', b').
 
-  Global Instance OccursCheckLawsPair {AT BT} `{OccursCheckLaws AT, OccursCheckLaws BT} :
-    OccursCheckLaws (Pair AT BT).
-  Proof.
-    constructor.
-    - intros. destruct t as [a b]; cbn.
-      now rewrite ?occurs_check_shift.
-    - intros ? ? ? [a b] [a' b']; cbn.
-      destruct (occurs_check xIn a) eqn:Heq1; intros; try discriminate.
-      destruct (occurs_check xIn b) eqn:Heq2; intros; try discriminate.
-      apply occurs_check_sound in Heq1.
-      apply occurs_check_sound in Heq2.
-      congruence.
-  Qed.
-
-  Global Instance OccursCheckOption {AT} `{OccursCheck AT} :
+  #[export] Instance occurs_check_option {AT} `{OccursCheck AT} :
     OccursCheck (Option AT) :=
     fun _ _ xIn ma =>
       match ma with
-      | Some a => option_map Some (occurs_check xIn a)
+      | Some a => option.map Some (occurs_check xIn a)
       | None   => Some None
       end.
 
-  Global Instance OccursCheckLawsOption {AT} `{OccursCheckLaws AT} :
-    OccursCheckLaws (Option AT).
+  #[export] Instance occurs_check_unit : OccursCheck Unit :=
+    fun _ _ _ t => match t with tt => Some tt end.
+
+  Definition OccursCheckShiftPoint {T} {subT : Subst T} {ocT : OccursCheck T} :
+    forall {Σ x} (xIn : x ∈ Σ) (t : T (Σ - x)), Prop :=
+    fun Σ x xIn t => wp (eq t) (occurs_check xIn (subst t (sub_shift xIn))).
+
+  Definition OccursCheckSoundPoint {T} {subT : Subst T} {ocT : OccursCheck T} :
+    forall {Σ x} (xIn : x ∈ Σ) (t : T Σ) , Prop :=
+    fun Σ x xIn t => wlp (fun t' => t = subst t' (sub_shift xIn)) (occurs_check xIn t).
+
+  Class OccursCheckLaws (T : LCtx -> Type) `{Subst T, OccursCheck T} : Prop :=
+    { occurs_check_shift {Σ x} (xIn : x ∈ Σ) (t : T (Σ - x)) : OccursCheckShiftPoint xIn t;
+      occurs_check_sound {Σ x} (xIn : x ∈ Σ) (t : T Σ) : OccursCheckSoundPoint xIn t;
+    }.
+  Global Arguments OccursCheckLaws T {_ _}.
+
+  Ltac occurs_check_mixin :=
+    match goal with
+    | H: ?P |- ?P => exact H
+    | |- ?x = ?x => refine eq_refl
+    | |- ?x = ?y =>
+        let hx := head x in
+        let hy := head y in
+        is_constructor hx; is_constructor hy;
+        first [ subst; refine eq_refl (* | f_equal *) ]
+    | |- wlp _ (occurs_check ?xIn ?t) =>
+        generalize (occurs_check_sound xIn t);
+        apply wlp_monotonic; intros ? ->
+    | |- wp _ (occurs_check ?xIn (subst ?t _)) =>
+        generalize (occurs_check_shift xIn t);
+        apply wp_monotonic; intros ? <-
+    | |- OccursCheckLaws _ =>
+        constructor; unfold OccursCheckShiftPoint, OccursCheckSoundPoint;
+        let x := fresh in
+        intros ? ? ? x; induction x
+    end.
+
+  Ltac occurs_check_derive :=
+    repeat
+      (try progress cbn;
+       first
+         [ option.tactics.mixin
+         | occurs_check_mixin]);
+    try progress cbn; try easy.
+  Local Ltac derive := occurs_check_derive.
+
+  Lemma occurs_check_env_shift_point {B : Set} {T : LCtx -> B -> Set}
+    {subT: forall b : B, Subst (fun Σ => T Σ b)}
+    {ocT : forall b : B, OccursCheck (fun Σ => T Σ b)}
+    {Σ : LCtx} {x} (xIn : x ∈ Σ)
+    {Γ : Ctx B} (ts : Env (T (Σ - x)) Γ) :
+    env.All (fun b => OccursCheckShiftPoint xIn) ts ->
+    OccursCheckShiftPoint xIn ts.
+  Proof. unfold OccursCheckShiftPoint. induction 1; derive. Qed.
+
+  Lemma occurs_check_env_sound_point {B : Set} {T : LCtx -> B -> Set}
+    {subT: forall b : B, Subst (fun Σ => T Σ b)}
+    {ocT : forall b : B, OccursCheck (fun Σ => T Σ b)}
+    {Σ : LCtx} {x} (xIn : x ∈ Σ)
+    {Γ : Ctx B} (ts : Env (T Σ) Γ) :
+    env.All (fun b t => OccursCheckSoundPoint xIn t) ts ->
+    OccursCheckSoundPoint xIn ts.
+  Proof. unfold OccursCheckSoundPoint; induction 1; derive. Qed.
+
+  #[export] Instance occurs_check_laws_term {τ} :
+    OccursCheckLaws (fun Σ => Term Σ τ).
   Proof.
-    constructor.
-    { intros. destruct t as [a|]; cbn.
-      - now rewrite ?occurs_check_shift.
-      - reflexivity.
-    }
-    { intros ? ? ? [a|] mt' Heq; cbn.
-      - apply option_map_eq_some' in Heq. destruct Heq as [t' [Heq <-]].
-        apply occurs_check_sound in Heq. subst. reflexivity.
-      - apply noConfusion_inv in Heq. cbn in Heq. subst. reflexivity.
-    }
+    derive.
+    - unfold sub_shift. rewrite env.lookup_tabulate. cbn.
+      now rewrite ctx.occurs_check_shift_var.
+    - generalize (occurs_check_env_shift_point IH).
+      apply wp_monotonic. intros ? <-. reflexivity.
+    - pose proof (ctx.occurs_check_var_spec xIn ςInΣ) as H.
+      destruct (ctx.occurs_check_var xIn ςInΣ); constructor; cbn.
+      destruct H as [H1 H2]. subst. unfold sub_shift.
+      now rewrite env.lookup_tabulate.
+    - generalize (occurs_check_env_sound_point IH).
+      apply wlp_monotonic. now intros ts' ->.
   Qed.
 
-  Global Instance OccursCheckUnit : OccursCheck Unit :=
-    fun _ _ _ _ => Some tt.
-  Global Instance OccursCheckLawsUnit : OccursCheckLaws Unit.
-  Proof.
-    constructor; cbn.
-    - destruct t; reflexivity.
-    - destruct t, t'; reflexivity.
-  Qed.
+  #[export] Instance occurs_check_laws_list {T : LCtx -> Type} `{OccursCheckLaws T} :
+    OccursCheckLaws (fun Σ => list (T Σ)).
+  Proof. derive. Qed.
+
+  #[export] Instance occurs_check_laws_env {I : Set} {T : LCtx -> I -> Set}
+   {_ : forall i : I, Subst (fun Σ => T Σ i)}
+   {_ : forall i : I, OccursCheck (fun Σ => T Σ i)}
+   {_ : forall i : I, OccursCheckLaws (fun Σ => T Σ i)}
+   {Γ : Ctx I} :
+    OccursCheckLaws (fun Σ => Env (T Σ) Γ).
+  Proof. derive. Qed.
+
+  #[export] Instance occurs_check_laws_sub {Σ} : OccursCheckLaws (Sub Σ) :=
+    occurs_check_laws_env.
+
+  #[export] Instance occurs_check_laws_pair {AT BT} `{OccursCheckLaws AT, OccursCheckLaws BT} :
+    OccursCheckLaws (Pair AT BT).
+  Proof. derive. Qed.
+
+  #[export] Instance occurs_check_laws_option {AT} `{OccursCheckLaws AT} :
+    OccursCheckLaws (Option AT).
+  Proof. derive. Qed.
+
+  #[export] Instance occurs_check_laws_unit : OccursCheckLaws Unit.
+  Proof. derive. Qed.
 
 End OccursCheckOn.
